theories/lang/cpp/logic/call.v
@@ -42,26 +42,35 @@ Section with_resolve.
                          Qarg free free' -* Q (a :: ps) ((free >*> free')%free :: frees))
     | _ , _ => False (* mismatched arguments and parameters. *)
     end.
-  #[program] Definition wp_args (ts : list type) (es : list Expr) (Q : list ptr -> FreeTemps -> mpred) : mpred :=
-    wp_args' ts es (fun ps (frees : list FreeTemps.t) => Q ps (λne x, ([∗list] f ∈ frees, (f : FreeTemps.t) emp) ** x)).
-  Next Obligation. solve_proper. Qed.
 
-  Lemma wp_args_frame_strong : forall ts es Q Q',
-      (Forall vs free, [| length vs = length es |] -* Q vs free -* Q' vs free) |-- wp_args ts es Q -* wp_args ts es Q'.
-  Proof. (*
+  Lemma wp_args'_frame_strong : forall ts es Q Q',
+      (Forall vs free, [| length vs = length es |] -* Q vs free -* Q' vs free) |-- wp_args' ts es Q -* wp_args' ts es Q'.
+  Proof.
     elim; destruct es => /=; try solve [ by intros; iIntros "? []" ].
     { by iIntros (? ?) "H"; iApply "H". }
-    { iIntros (? ?) "H" => /wp_args/=.  iIntros (?) "at".
-      iDestruct ("K" with "at") as (Qarg) "K".
+    { iIntros (? ?) "H". iIntros "K" (p).
+      iDestruct ("K" $! p) as (Qarg) "K".
       iExists _.
       iDestruct "K" as "[$ K]".
       iRevert "K"; iApply H.
       iIntros (?? ?) "X".
-      iIntros (?) "f".
+      iIntros (??) "f".
       iDestruct ("X" with "f") as "X".
       iRevert "X"; iApply "H".
       iPureIntro; simpl; eauto. }
-  Qed. *) Admitted.
+  Qed.
+
+  Definition pars := fold_right FreeTemps.par FreeTemps.id.
+
+  #[program] Definition wp_args (ts : list type) (es : list Expr) (Q : list ptr -> FreeTemps -> mpred) : mpred :=
+    wp_args' ts es (fun ps (frees : list FreeTemps.t) => Q ps (pars frees)).
+
+  Lemma wp_args_frame_strong : forall ts es Q Q',
+      (Forall vs free, [| length vs = length es |] -* Q vs free -* Q' vs free) |-- wp_args ts es Q -* wp_args ts es Q'.
+  Proof.
+    intros. iIntros "X"; iApply wp_args'_frame_strong.
+    iIntros (??) "?". by iApply "X".
+  Qed.
 
   Lemma wp_args_frame : forall ts es Q Q',
       (Forall vs free, Q vs free -* Q' vs free) |-- wp_args ts es Q -* wp_args ts es Q'.
